 Theorem â€œAddingâ‚‚â€:
      m = mâ‚€ âˆ§ n = nâ‚€
    â‡’â…  while m â‰  0
          do
            m := m - 1 â®
            n := n + 1
          od
      â†
      n = mâ‚€ + nâ‚€
Proof:
    m = mâ‚€ âˆ§ n = nâ‚€
  â‰¡âŸ¨ â€œIdentity of +â€ âŸ© 
    m = mâ‚€ âˆ§ n + 0 = nâ‚€ + 0
  â‰¡âŸ¨ â€œUnary minusâ€ âŸ© 
    m = mâ‚€ âˆ§ n + m + - m = nâ‚€ + m + - m
  â‰¡âŸ¨ â€œCancellation of +â€ âŸ©
    m = mâ‚€ âˆ§ n + m = nâ‚€ + m
  â‰¡âŸ¨ â€œAbbreviated replacementâ€, substitution âŸ©
    m = mâ‚€ âˆ§ n + m = nâ‚€ + mâ‚€    
  â‡’âŸ¨ â€œWeakeningâ€ âŸ©
    m + n = mâ‚€ + nâ‚€
  â‡’â…  while m â‰  0
          do
            m := m - 1 â®
            n := n + 1
          od
      â† 
  
  âŸ¨ â€œWhileâ€ with subproof:
              (m â‰  0) âˆ§ (m + n = mâ‚€ + nâ‚€)
            â‡’âŸ¨ â€œStrengtheningâ€ âŸ©
              (m + n = mâ‚€ + nâ‚€)
            =âŸ¨ â€œIdentity of +â€ âŸ©
              (m + 0 + n = mâ‚€ + nâ‚€)
            =âŸ¨ â€œUnary minusâ€ âŸ© 
              (m + - 1 + 1 + n = mâ‚€ + nâ‚€)
            =âŸ¨ â€œSubtractionâ€ âŸ©
              (m - 1 + 1 + n = mâ‚€ + nâ‚€) 
            =âŸ¨ â€œSymmetry of +â€ âŸ©
              (m - 1 + n + 1 = mâ‚€ + nâ‚€)              
            â‡’â… m := m - 1 â† âŸ¨ â€œAssignmentâ€ with Substitution âŸ©
              (m + n + 1 = mâ‚€ + nâ‚€)
            â‡’â… n := n + 1 â† âŸ¨ â€œAssignmentâ€ with Substitution âŸ©
              m + n = mâ‚€ + nâ‚€
    âŸ©
    Â¬ (m â‰  0) âˆ§ (m + n = mâ‚€ + nâ‚€) 
  =âŸ¨ â€œDefinition of â‰ â€ âŸ©  
    Â¬ Â¬ (m = 0) âˆ§ (m + n = mâ‚€ + nâ‚€) 
  =âŸ¨ â€œDouble negationâ€ âŸ©
    (m = 0) âˆ§ (m + n = mâ‚€ + nâ‚€) 
  =âŸ¨ â€œAbbreviated replacementâ€, Substitution âŸ©
    (m = 0) âˆ§ (0 + n = mâ‚€ + nâ‚€) 
  â‡’âŸ¨ â€œWeakeningâ€ âŸ©   
    (0 + n = mâ‚€ + nâ‚€) 
  =âŸ¨ â€œIdentity of +â€ âŸ© 
    n = mâ‚€ + nâ‚€
    
------------------

Theorem â€œAnswering...â€:
      true
    â‡’â…  i := 0 â®
        while i = 0
          do
            n := n + 1
          od
      â†
      n = 42
Proof:
    true
  =âŸ¨ â€œReflexivity of =â€ âŸ©
    (0 = 0)
  =âŸ¨ Substitution âŸ©
    (i = 0) [i â‰” 0]
  â‡’â… i := 0 â†âŸ¨â€œAssignmentâ€âŸ©
    i = 0
  â‡’â…
        while i = 0
          do
            n := n + 1
          od
      â† 
   âŸ¨ â€œWhileâ€ with subproof:
          i = 0 âˆ§ i = 0
        =âŸ¨ â€œIdempotency of âˆ§â€ âŸ©
          i = 0
        = âŸ¨ Substitution âŸ©
          (i = 0)[n â‰” n + 1]
        â‡’â… n := n + 1 â† âŸ¨â€œAssignmentâ€âŸ©                             
           i = 0
    âŸ©
    Â¬(i = 0) âˆ§ (i = 0)
  =âŸ¨ â€œContradictionâ€ âŸ©
    false
  â‡’âŸ¨ â€œex falso quodlibetâ€ âŸ©
    n = 42   
              
---------------------

Theorem (13.14) â€œSnoc is not emptyâ€:  xs â–¹ x â‰  ğœ–
Proof:
  By induction on `xs : Seq A`:
    Base case `ğœ– â–¹ x â‰  ğœ–`:
        ğœ– â–¹ x â‰  ğœ–
      =âŸ¨ â€œDefinition of â‰ â€ âŸ©
        Â¬ (ğœ– â–¹ x = ğœ–)
      =âŸ¨ â€œDefinition of â–¹ for ğœ–â€ âŸ©
        Â¬ (x â—ƒ ğœ– = ğœ–)
      =âŸ¨ â€œCons is not emptyâ€ âŸ©
        Â¬ false
      =âŸ¨ â€œNegation of `false`â€ âŸ©
        true        
    Induction step `âˆ€ y : A â€¢ (y â—ƒ xs) â–¹ x â‰  ğœ–`:
      For any `y : A`:
          (y â—ƒ xs) â–¹ x â‰  ğœ–
        =âŸ¨ â€œDefinition of â–¹ for â—ƒâ€ âŸ©
          y â—ƒ (xs â–¹ x) â‰  ğœ–
        =âŸ¨ â€œDefinition of â‰ â€ âŸ©
          Â¬ (y â—ƒ (xs â–¹ x) = ğœ–)
        =âŸ¨ â€œCons is not emptyâ€ âŸ©
          Â¬ false
        =âŸ¨ â€œNegation of `false`â€ âŸ©
          true

--------------
Theorem (13.19) â€œRight-identity of âŒ¢â€:
    xs âŒ¢ ğœ– = xs
Proof:
  By induction on `xs : Seq A`:
    Base case:
        ğœ– âŒ¢ ğœ–  
      =âŸ¨ â€œLeft-identity of âŒ¢â€ âŸ©
        ğœ–
    Induction step:
      For any `y : A`:
          (y â—ƒ xs) âŒ¢ ğœ–
        =âŸ¨ â€œMutual associativity of â—ƒ with âŒ¢â€ âŸ©
          y â—ƒ (xs âŒ¢ ğœ–)
        =âŸ¨ Induction hypothesis âŸ©
          y â—ƒ xs
----------------          

Theorem (11.7) (11.7s) â€œSimple Membershipâ€:
   e âˆˆ { x â™ P }  â‰¡ P[x â‰” e]
Proof:
    e âˆˆ { x â™ P }
  â‰¡âŸ¨ â€œSet Abbreviationâ€ âŸ©
    e âˆˆ { x â™ P â€¢ x }
  â‰¡âŸ¨ â€œSet membershipâ€ âŸ©
    âˆƒ x â™ P â€¢ e = x
  â‰¡âŸ¨ â€œTrading for âˆƒâ€ âŸ©
    âˆƒ x â€¢ P âˆ§ e = x
  â‰¡âŸ¨ â€œSymmetry of âˆ§â€ âŸ©
    âˆƒ x â€¢ e = x âˆ§ P
  â‰¡âŸ¨ â€œSymmetry of =â€ âŸ©
    âˆƒ x â€¢ x = e âˆ§ P
  â‰¡âŸ¨ â€œTrading for âˆƒâ€ âŸ©
    âˆƒ x â™ x = e â€¢ P
  â‰¡âŸ¨ â€œOne-point rule for âˆƒâ€ âŸ©
    P[x â‰” e]

 --------------

Theorem â€œM2.3bâ€:   R â–· B = R â¨¾ id B
   Proof:
    Using â€œRelation extensionalityâ€:
      For any `a, d`:
          a â¦— R â–· B â¦˜ d
        â‰¡âŸ¨ â€œRange restrictionâ€ âŸ©
          a â¦— R â¦˜ d âˆˆ B
        â‰¡âŸ¨ Substitution âŸ© 
          (a â¦— R â¦˜ b)[b â‰” d âˆˆ B]
        â‰¡âŸ¨ â€œOne-point rule for âˆƒâ€ âŸ© 
          âˆƒ b â™ b = d âˆˆ B â€¢ a â¦— R â¦˜ b
        â‰¡âŸ¨ â€œTrading for âˆƒâ€ âŸ©
          âˆƒ b â€¢ b = d âˆˆ B âˆ§ a â¦— R â¦˜ b 
        â‰¡âŸ¨ â€œSymmetry of âˆ§â€ âŸ©
          âˆƒ b â€¢ a â¦— R â¦˜ b âˆ§ b = d âˆˆ B
        â‰¡âŸ¨ â€œRelationship via `id`â€ âŸ©
          âˆƒ b â€¢ a â¦— R â¦˜ b âˆ§ b â¦— id B â¦˜ d  
        â‰¡âŸ¨ â€œRelation compositionâ€ âŸ©
        a â¦— R â¨¾ id B â¦˜ d 
-----------
Theorem (14.231) â€œDomain of â—â€: Dom (A â— R) = A âˆ© Dom R
Proof:
  Using â€œSet extensionalityâ€:
    Subproof for `âˆ€ e â€¢ e âˆˆ Dom (A â— R) â‰¡ e âˆˆ A âˆ© Dom R`:
      For any `e`:
          e âˆˆ Dom (A â— R)
        =âŸ¨ â€œMembership in `Dom`â€ âŸ©
          (âˆƒ y â€¢ e â¦— A â— R â¦˜ y)
        =âŸ¨ â€œDefinition of â—â€ âŸ©
          (âˆƒ y â€¢ e â¦— R âˆ© (A Ã— ğ”) â¦˜ y)
        =âŸ¨ â€œRelation intersectionâ€ âŸ©
          (âˆƒ y â€¢ e â¦— R â¦˜ y âˆ§ e â¦— A Ã— ğ” â¦˜ y)
        =âŸ¨ â€œRelationship via Ã—â€ âŸ©
          (âˆƒ y â€¢ e â¦— R â¦˜ y âˆ§ (e âˆˆ A âˆ§ y âˆˆ ğ”))
        =âŸ¨ â€œUniversal setâ€ , â€œIdentity of âˆ§â€ âŸ©
          (âˆƒ y â€¢ e â¦— R â¦˜ y âˆ§ e âˆˆ A)
        =âŸ¨ â€œDistributivity of âˆ§ over âˆƒâ€ âŸ©
          e âˆˆ A âˆ§ (âˆƒ y â€¢ e â¦— R â¦˜ y)
        =âŸ¨ â€œDistributivity of âˆ§ over âˆƒâ€ âŸ©
          e âˆˆ A âˆ§ (âˆƒ y â€¢ e â¦— R â¦˜ y)
        =âŸ¨ â€œMembership in `Dom`â€ âŸ©
          e âˆˆ Dom R âˆ§ e âˆˆ A
        =âŸ¨ â€œSymmetry of âˆ§â€ âŸ©
          e âˆˆ A âˆ§ e âˆˆ Dom R
        =âŸ¨ â€œIntersectionâ€ âŸ©
          e âˆˆ A âˆ© Dom R
 ---------

Theorem â€œM2.2â€:
      m = mâ‚€ âˆ§ n = nâ‚€
    â‡’â…  while n â‰  0
          do
            n := n - 1 â®
            m := m - 1
          od
      â†
      m = mâ‚€ - nâ‚€
Proof:
    m = mâ‚€ âˆ§ n = nâ‚€   â•â•â•  Precondition
  â‰¡âŸ¨ â€œCancellation of +â€, â€œSubtractionâ€ âŸ©
    m - n = mâ‚€ - n âˆ§ n = nâ‚€
  â‰¡âŸ¨ â€œSymmetry of âˆ§â€ âŸ©
    n = nâ‚€ âˆ§ m - n = mâ‚€ - n
  â‰¡âŸ¨ Substitution âŸ©
    n = nâ‚€ âˆ§ (m - n = mâ‚€ - z)[z â‰” n]
  â‰¡âŸ¨ â€œReplacementâ€, Substitution âŸ©
    n = nâ‚€ âˆ§ (m - n = mâ‚€ - nâ‚€)
  â‡’âŸ¨ â€œWeakeningâ€ âŸ©
    m - n = mâ‚€ - nâ‚€
  â‡’â… while n â‰  0 do
        n := n - 1 â®
        m := m - 1
      od â†âŸ¨ â€œWhileâ€ with subproof:
          n â‰  0 âˆ§ m - n = mâ‚€ - nâ‚€  â•â•â•  Loop condition and invariant
        â‡’ âŸ¨ â€œWeakeningâ€ âŸ©
          m - n = mâ‚€ - nâ‚€
        â‰¡âŸ¨ â€œIdentity of +â€ âŸ©
          m - n + 0 = mâ‚€ - nâ‚€
        â‰¡âŸ¨ Fact `1 - 1 = 0` âŸ©
          m - n + (1 - 1) = mâ‚€ - nâ‚€
        â‰¡âŸ¨ â€œSubtractionâ€ âŸ©
          m + - n + (1 + - 1) = mâ‚€ - nâ‚€
        â‰¡âŸ¨ â€œSymmetry of +â€ âŸ©
          m + 1 + - n + - 1 = mâ‚€ - nâ‚€
        â‰¡âŸ¨ â€œSubtractionâ€ âŸ©
          m + 1 - n - 1 = mâ‚€ - nâ‚€
        â‰¡âŸ¨ â€œSubtraction of additionâ€âŸ©
          (m + 1) - (n + 1) = mâ‚€ - nâ‚€
        â‰¡âŸ¨ (15.26) âŸ©
          (m - 1) - (n - 1) = mâ‚€ - nâ‚€
        â‡’â… n := n - 1 â†âŸ¨ â€œAssignmentâ€ with substitution âŸ©
          (m - 1) - n = mâ‚€ - nâ‚€
        â‡’â… m := m - 1 â†âŸ¨ â€œAssignmentâ€ with substitution âŸ©
          m - n = mâ‚€ - nâ‚€
    âŸ©
    Â¬ (n â‰  0) âˆ§ m - n = mâ‚€ - nâ‚€  â•â•â• Negated loop condition, and invariant
  =âŸ¨ â€œDefinition of â‰ â€ âŸ©
    Â¬ Â¬ (n = 0) âˆ§ m - n = mâ‚€ - nâ‚€
  =âŸ¨ â€œDouble negationâ€ âŸ©
    n = 0 âˆ§ m - n = mâ‚€ - nâ‚€
  =âŸ¨ Substitution âŸ©
    n = 0 âˆ§ (m - z = mâ‚€ - nâ‚€)[z â‰” n]
  =âŸ¨ â€œReplacementâ€ with Substitution âŸ©
    n = 0 âˆ§ (m - 0 = mâ‚€ - nâ‚€)
  â‡’âŸ¨ â€œWeakeningâ€ âŸ©
    m - 0 = mâ‚€ - nâ‚€
  =âŸ¨ â€œRight-identity of -â€ âŸ©
    m = mâ‚€ - nâ‚€

Theorem â€œM2.3bâ€: Ran (R â¨¾ S) = Ran (Ran R â— S)
Proof:
  Using â€œSet extensionalityâ€:
    For any `y`:
        y âˆˆ Ran (R â¨¾ S) 
      =âŸ¨â€œMembership in `Ran`â€âŸ© 
        âˆƒ x â€¢ x â¦— R â¨¾ S â¦˜ y 
      =âŸ¨ â€œRelation compositionâ€ âŸ© 
        âˆƒ x â€¢ (âˆƒ b â€¢ x â¦— R â¦˜ b âˆ§ b â¦— S â¦˜ y ) 
      =âŸ¨ â€œTrading for âˆƒâ€ âŸ© 
        âˆƒ x â€¢ (âˆƒ b â™ x â¦— R â¦˜ b â€¢ b â¦— S â¦˜ y )
      =âŸ¨ â€œNesting for âˆƒâ€ âŸ© 
        âˆƒ x, b â™ x â¦— R â¦˜ b â€¢ b â¦— S â¦˜ y 
      =âŸ¨ â€œDummy list permutation for âˆƒâ€ âŸ© 
        âˆƒ b, x â™ x â¦— R â¦˜ b â€¢ b â¦— S â¦˜ y 
      =âŸ¨ â€œNesting for âˆƒâ€ âŸ© 
        âˆƒ b â€¢ (âˆƒ x â™ x â¦— R â¦˜ b â€¢ b â¦— S â¦˜ y)
      =âŸ¨ (9.22) âŸ© 
        âˆƒ b â€¢ ((b â¦— S â¦˜ y) âˆ§ (âˆƒ x  â€¢  x â¦— R â¦˜ b))
      =âŸ¨ â€œMembership in `Ran`â€ âŸ© 
        âˆƒ b â€¢ ((b â¦— S â¦˜ y) âˆ§ (b âˆˆ Ran R))
      =âŸ¨ â€œRelationship via â—â€ âŸ© 
        âˆƒ b â€¢ (b â¦— Ran R â— S â¦˜ y)
      =âŸ¨ â€œMembership in `Ran`â€ âŸ© 
        y âˆˆ Ran (Ran R â— S )

Theorem â€œM2.3aâ€:   A â— R = id A â¨¾ R
Proof:
  Using â€œRelation extensionalityâ€:
    For any `x, y`:
        x â¦— A â— R â¦˜ y
      â‰¡âŸ¨ â€œDomain restrictionâ€ âŸ©
        x âˆˆ A âˆ§ x â¦— R â¦˜ y
      â‰¡âŸ¨ â€œIdentity of â¨¾â€ âŸ©
        x âˆˆ A âˆ§ x â¦— ğ•€ â¨¾ R â¦˜ y
      â‰¡âŸ¨ â€œRelation compositionâ€ âŸ©
        x âˆˆ A âˆ§ (âˆƒ b â€¢ x â¦— ğ•€ â¦˜ b âˆ§ b â¦— R â¦˜ y )
      â‰¡âŸ¨ â€œRelationship via ğ•€â€ âŸ©
        x âˆˆ A âˆ§ (âˆƒ b â€¢ x = b âˆ§ b â¦— R â¦˜ y )
      â‰¡âŸ¨ â€œTrading for âˆƒâ€ âŸ©
        x âˆˆ A âˆ§ (âˆƒ b â™ x = b â€¢ b â¦— R â¦˜ y )
      â‰¡âŸ¨ â€œDistributivity of âˆ§ over âˆƒâ€ âŸ©
        (âˆƒ b â™ x = b â€¢ x âˆˆ A âˆ§ b â¦— R â¦˜ y)
      â‰¡âŸ¨ â€œTrading for âˆƒâ€ âŸ©
        (âˆƒ b â€¢ x = b âˆ§ x âˆˆ A âˆ§ b â¦— R â¦˜ y)
      â‰¡âŸ¨ â€œAssociativity of âˆ§â€ âŸ©
        (âˆƒ b â€¢ x = b âˆ§ x âˆˆ A âˆ§ b â¦— R â¦˜ y)
      â‰¡âŸ¨ Substitution âŸ©
        âˆƒ b â€¢ x = b âˆ§ (g âˆˆ A âˆ§ b â¦— R â¦˜ y)[g â‰” x]
      â‰¡âŸ¨ â€œReplacementâ€ with Substitution âŸ©
        âˆƒ b â€¢ x = b âˆ§ b âˆˆ A âˆ§ b â¦— R â¦˜ y
      â‰¡âŸ¨ â€œReplacementâ€ with Substitution âŸ©
        âˆƒ b â€¢ x = b âˆ§ b âˆˆ A âˆ§ b â¦— R â¦˜ y
      â‰¡âŸ¨ â€œIdempotency of âˆ§â€ âŸ©
        âˆƒ b â€¢ x = b âˆˆ A âˆ§ b â¦— R â¦˜ y
      â‰¡âŸ¨ â€œRelationship via `id`â€ âŸ©
        âˆƒ b â€¢ x â¦— id A â¦˜ b âˆ§ b â¦— R â¦˜ y
      â‰¡âŸ¨ â€œRelation compositionâ€ âŸ©
        x â¦— id A â¨¾ R â¦˜ y

Theorem â€œPredecessor of non-zeroâ€:
    n â‰  0  â‰¡  suc (pred n) = n
Proof:
  By induction on `n : â„•`:
    Base case `0 â‰  0  â‰¡  suc (pred 0) = 0`:
        suc (pred 0) = 0
      =âŸ¨ â€œPredecessor of zeroâ€ âŸ©
        suc 0 = 0
      =âŸ¨ â€œZero is not successorâ€ âŸ©
        false
      =âŸ¨ â€œIrreflexivity of â‰ â€ âŸ©
        0 â‰  0    
    Induction step `suc n â‰  0  â‰¡  suc (pred (suc n)) = suc n`:
        suc n â‰  0  â‰¡  suc (pred (suc n)) = suc n
      = âŸ¨ â€œPredecessor of successorâ€ âŸ©
        suc n â‰  0  â‰¡  suc n = suc n
      = âŸ¨ â€œReflexivity of =â€ âŸ©
        suc n â‰  0 â‰¡ true
      =âŸ¨ â€œDefinition of â‰ â€ âŸ©
        Â¬ (suc n = 0) â‰¡ true
      =âŸ¨ â€œZero is not successorâ€ âŸ©
        Â¬ (false) â‰¡ true
      =âŸ¨ â€œNegation of `false`â€ âŸ©
        true â‰¡ true
      =âŸ¨ â€œIdentity of â‰¡â€ âŸ©
        true

Theorem â€œM2.1bâ€:
    reflexive E  âˆ§  univalent F  âˆ§  E âŠ† F â¨¾ F Ë˜
  â‡’ E â¨¾ F = F
Proof:
  Assuming `reflexive E` and using with â€œDefinition of univalenceâ€,
           `univalent F` and using with â€œDefinition of univalenceâ€,
           `E âŠ† F â¨¾ F Ë˜`:
    Using â€œMutual inclusionâ€:
      Subproof for `E â¨¾ F âŠ† F`:
            E â¨¾ F
        âŠ†âŸ¨ â€œMonotonicity of â¨¾â€ with Assumption `E âŠ† F â¨¾ F Ë˜` âŸ©
            (F â¨¾ F Ë˜) â¨¾ F
        =âŸ¨ â€œAssociativity of â¨¾â€ âŸ©
            F â¨¾ (F Ë˜ â¨¾ F)
        âŠ†âŸ¨ â€œMonotonicity of â¨¾â€ with Assumption `univalent F` âŸ©
            F â¨¾ ğ•€
        =âŸ¨ â€œIdentity of â¨¾â€ âŸ©
            F
      Subproof for `F âŠ† E â¨¾ F`:
        Using â€œRelation inclusionâ€:
          Subproof for `âˆ€ x â€¢ (âˆ€ y â€¢ x â¦— F â¦˜ y â‡’ x â¦— E â¨¾ F â¦˜ y )`:
            For any `x`, `y`:
                x â¦— F â¦˜ y â‡’ x â¦— E â¨¾ F â¦˜ y
              =âŸ¨ â€œRelation compositionâ€ âŸ©
                x â¦— F â¦˜ y â‡’ (âˆƒ b â€¢ x â¦— E â¦˜ b âˆ§ b â¦— F â¦˜ y )
              =âŸ¨ â€œRelation compositionâ€ âŸ©
                x â¦— F â¦˜ y â‡’ (âˆƒ b â€¢ x â¦— E â¦˜ b âˆ§ b â¦— F â¦˜ y )
              â‡’âŸ¨ ?, â€œTrading for âˆƒâ€ âŸ©
                âˆƒ z â€¢ x â¦— E â¦˜ z âˆ§ z â¦— F â¦˜ y
              â‡’âŸ¨ â€œRelation compositionâ€ âŸ©
                x â¦— E â¨¾ F â¦˜ y
Theorem â€œM2.1aâ€: R = R â¨¾ (ğ•€ âˆ© R Ë˜ â¨¾ R)
Proof:
  Using â€œMutual inclusionâ€:
    Subproof for `R âŠ† R â¨¾ (ğ•€ âˆ© R Ë˜ â¨¾ R)`:
        R â¨¾ (ğ•€ âˆ© R Ë˜ â¨¾ R)
      âŠ‡âŸ¨â€œModal ruleâ€âŸ©
        (R) â¨¾ ğ•€  âˆ© R
      =âŸ¨â€œIdentity of â¨¾â€âŸ©
        (R) â¨¾ ğ•€  âˆ© R â¨¾ ğ•€
      =âŸ¨â€œIdempotency of âˆ©â€âŸ©
        (R) â¨¾ ğ•€ 
      =âŸ¨â€œIdentity of â¨¾â€âŸ©
        R
    Subproof for `R â¨¾ (ğ•€ âˆ© R Ë˜ â¨¾ R)  âŠ† R `:
        R â¨¾ (ğ•€ âˆ© R Ë˜ â¨¾ R)
      âŠ†âŸ¨ â€œSub-distributivity of â¨¾ over âˆ©â€ âŸ©
        R â¨¾ ğ•€ âˆ© R â¨¾ (R Ë˜ â¨¾ R)
      =âŸ¨ â€œIdentity of â¨¾â€ âŸ©
        R âˆ© (R â¨¾ R Ë˜ â¨¾ R)
      =âŸ¨ â€œSet inclusion via âˆ©â€ with â€œCo-difunctionalityâ€ âŸ©
        R
Theorem â€œSymmetry of +â€: âˆ€ m â€¢ âˆ€ n â€¢ m + n = n + m
Proof:
  Using â€œInduction over â„•â€:
    Subproof:
      For any `n : â„•`:
          0 + n
        =âŸ¨ â€œDefinition of +â€ âŸ©
          n
        =âŸ¨ â€œRight-identity of +â€  âŸ©
          n + 0
    Subproof:
      For any `m : â„•` satisfying â€œIndHypâ€ `âˆ€ n â€¢ m + n = n + m`:
        For any `n : â„•`:
            (m + 1) + n
          =âŸ¨ â€œDefinition of +â€ âŸ©
            (m + n) + 1
          =âŸ¨ Assumption â€œIndHypâ€ âŸ©
            (n + m) + 1
          =âŸ¨ â€œDefinition of +â€ âŸ©
            (n + 1) + m
          =âŸ¨ â€œShifting successor over +â€ âŸ©
            n + (m + 1)
Theorem â€œUnivalence of compositionâ€:
     univalent R â‡’ univalent S â‡’ univalent (R â¨¾ S)
Proof:
  Assuming `univalent R` and using with â€œDefinition of univalenceâ€,
           `univalent S` and using with â€œDefinition of univalenceâ€:
    Using â€œDefinition of univalenceâ€:
        (R â¨¾ S) Ë˜ â¨¾ (R â¨¾ S)
      =âŸ¨ â€œConverse of â¨¾â€ âŸ©
        (S Ë˜ â¨¾ R Ë˜) â¨¾ R â¨¾ S
      =âŸ¨ â€œAssociativity of â¨¾â€ âŸ©
        S Ë˜ â¨¾ (R Ë˜ â¨¾ R) â¨¾ S
      âŠ†âŸ¨ â€œMonotonicity of â¨¾â€ with â€œMonotonicity of â¨¾â€ with
         Assumption `univalent R` âŸ©
        S Ë˜ â¨¾ ğ•€ â¨¾ S
      =âŸ¨ â€œIdentity of â¨¾â€ âŸ©
        S Ë˜ â¨¾ S
      âŠ†âŸ¨ Assumption `univalent S` âŸ©
        ğ•€
Theorem â€œSquaringâ€:
      true
    â‡’â…  i := 0 â®
        s := 0 â®
        d := 1 â®
        while i â‰  n
          do
            s := s + d â®
            d := d + 2 â®
            i := i + 1
          od
       â† s = n Â· n
Proof:
    true   â•â•â•  Precondition
  â‰¡âŸ¨ â€œIdempotency of âˆ§â€ âŸ©
    true âˆ§ true 
  â‰¡âŸ¨ Fact `1 = 0 + 0 + 1`, Fact `0 = 0 Â· 0` âŸ©
    1 = 0 + 0 + 1 âˆ§ 0 = 0 Â· 0
  â‡’â… i := 0 â†âŸ¨ â€œAssignmentâ€ with substitution âŸ©
    1 = i + i + 1 âˆ§ 0 = i Â· i
  â‡’â… s := 0 â†âŸ¨ â€œAssignmentâ€ with substitution âŸ©
    1 = i + i + 1 âˆ§ s = i Â· i
  â‡’â… d := 1 â†âŸ¨ â€œAssignmentâ€ with substitution âŸ©
    d = i + i + 1 âˆ§ s = i Â· i      â•â•â•  Invariant
  â‡’â… while i â‰  n do
        s := s + d â®
        d := d + 2 â®
        i := i + 1
      od â†âŸ¨ â€œWhileâ€ with subproof:
          i â‰  n âˆ§ d = i + i + 1 âˆ§ s = i Â· i  â•â•â•  Loop condition and invariant
        â‡’âŸ¨ â€œWeakeningâ€ (3.76b) âŸ©
          d = i + i + 1 âˆ§ s = i Â· i
        =âŸ¨ â€œCancellation of +â€ âŸ©   
          d = i + i + 1 âˆ§ s + d = i Â· i + d
        =âŸ¨ Substitution âŸ© 
          d = i + i + 1 âˆ§ (s + d = i Â· i + z)[z â‰” d]
        â‰¡âŸ¨ â€œReplacementâ€ (3.84a) âŸ© 
          d = i + i + 1 âˆ§ (s + d = i Â· i + z)[z â‰” i + i + 1]
        â‡’â… s := s + d â†âŸ¨ â€œAssignmentâ€ with substitution âŸ©
          d = i + i + 1 âˆ§ s = i Â· i + i + i + 1
        â‰¡âŸ¨ â€œCancellation of +â€ âŸ©
          d + 2 = i + i + 1 + 2 âˆ§ s = i Â· i + i + i + 1
        â‡’â… d := d + 2 â†âŸ¨ â€œAssignmentâ€ with substitution âŸ©
          d = i + i + 1 + 2 âˆ§ s = i Â· i + i + i + 1
        â‰¡âŸ¨ â€œDistributivity of Â· over +â€, â€œIdentity of Â·â€ âŸ©
          d = i + i + 1 + 2 âˆ§ s = (i + 1) Â· (i + 1)
        â‡’â… i := i + 1 â†âŸ¨ â€œAssignmentâ€ with substitution
                         and Fact `1 + 1 = 2` âŸ©
          d = i + i + 1 âˆ§ s = i Â· i   â•â•â•  Invariant
    âŸ©
    Â¬ (i â‰  n) âˆ§ d = i + i + 1 âˆ§ s = i Â· i  â•â•â• Negated loop condition, and invariant
  â‰¡âŸ¨ â€œDefinition of â‰ â€, â€œDouble negationâ€ âŸ©
    (i = n) âˆ§ d = i + i + 1 âˆ§ s = i Â· i
  â‡’âŸ¨ â€œWeakeningâ€  (3.76b) âŸ©
    (i = n) âˆ§ s = i Â· i
  =âŸ¨ Substitution âŸ©
     i = n  âˆ§ (s = z Â· z)[z â‰” i]
  =âŸ¨ â€œReplacementâ€ (3.84a) , Substitution âŸ©
     i = n  âˆ§ s = n Â· n
  â‡’âŸ¨ â€œWeakeningâ€ (3.76b) âŸ© 
    s = n Â· n    â•â•â•  Postcondition

Theorem â€œSumming upâ€:
      true
    â‡’â…  s := 0 â®
        i := 0 â®
        while i â‰  n
          do
            s := s + f i â®
            i := i + 1
          od
      â†
      s = âˆ‘ j : â„• â™ j < n â€¢ f j
Proof:
    true
  =âŸ¨ â€œReflexivity of =â€ âŸ© 
    0 = 0
  =âŸ¨ â€œNothing is less than zeroâ€ , â€œEmpty range for âˆ‘â€ âŸ© 
    0 = âˆ‘ j : â„• â™ j < 0 â€¢ f j
  â‡’â… s := 0 â†âŸ¨ â€œAssignmentâ€ with substitution âŸ©
    s = âˆ‘ j : â„• â™ j < 0 â€¢ f j
  â‡’â… i := 0 â†âŸ¨ â€œAssignmentâ€ with substitution âŸ© 
    s = âˆ‘ j : â„• â™ j < i â€¢ f j
  â‡’â… while i â‰  n do
        s := s + f i â®
        i := i + 1
      od â†âŸ¨ â€œWhileâ€ with subproof:
          i â‰  n âˆ§ s = âˆ‘ j : â„• â™ j < i â€¢ f j  â•â•â•  Loop condition and invariant
        â‡’âŸ¨ â€œWeakeningâ€ (3.76b) âŸ© 
          s = (âˆ‘ j : â„• â™ j < i â€¢ f j) 
        =âŸ¨ Substitution, â€œCancellation of +â€ âŸ© 
          s + f i = (âˆ‘ j : â„• â™ j < i â€¢ f j) + (f j)[j â‰” i]
        =âŸ¨ â€œSplit off term from âˆ‘ at topâ€ âŸ©
          s + f i = âˆ‘ j : â„• â™ j < suc i â€¢ f j
        =âŸ¨ â€œSuccessorâ€ âŸ©    
          s + f i = âˆ‘ j : â„• â™ j < i + 1 â€¢ f j
        â‡’â… s := s + f i â†âŸ¨ â€œAssignmentâ€ with substitution âŸ©
          s = âˆ‘ j : â„• â™ j < i + 1 â€¢ f j       
        â‡’â… i := i + 1 â†âŸ¨ â€œAssignmentâ€ with substitution âŸ©
          s = âˆ‘ j : â„• â™ j < i â€¢ f j   â•â•â•  Invariant
    âŸ© 
    Â¬ (i â‰  n) âˆ§ s = âˆ‘ j : â„• â™ j < i â€¢ f j
  =âŸ¨ â€œDefinition of â‰ â€, â€œDouble negationâ€ âŸ©
    (i = n) âˆ§ s = âˆ‘ j : â„• â™ j < i â€¢ f j 
  =âŸ¨ Substitution âŸ©
    (i = n) âˆ§ (s = âˆ‘ j : â„• â™ j < z â€¢ f j)[z â‰” i]
  =âŸ¨ â€œReplacementâ€ (3.84a) , Substitution âŸ©
    (i = n) âˆ§ (s = âˆ‘ j : â„• â™ j < n â€¢ f j)
  â‡’âŸ¨ â€œWeakeningâ€ (3.76b) âŸ©
    s = âˆ‘ j : â„• â™ j < n â€¢ f j 

